\documentclass{article}
\usepackage{amsmath}
\usepackage{amssymb} %\mathbb

\begin{document}
  \title{Useful Sums}
  \author{Y. Lifanov}
  \date{\today}
  \maketitle

  For $n,m\in\mathbb{Z} \:: 0\leq m\leq n$,
  \begin{equation}
    \begin{aligned}
      \sum_{i = 0}^m\sum_{j = 0}^n\min\{i, j\} 
      &= 
      \sum_{i = 0}^m\sum_{j = 0}^i j + 
      \sum_{i = 0}^m\sum_{j = i + 1}^n i \\
      &= 
      \frac{1}{2}\sum_{i = 0}^m i(i + 1) + 
      \sum_{i = 0}^m i(n - i) \\
      &= 
      \left(n + \frac{1}{2}\right)\sum_{i = 0}^m i - 
      \frac{1}{2}\sum_{i = 0}^m i^2 \\
      &=
      \frac{1}{6}m(m + 1)\left(3n - m + 1\right).
    \end{aligned}
  \end{equation}

  For $n,m\in\mathbb{Z} \:: 0\leq m\leq n$ and $x\in\mathbb{Z}$,
  \begin{equation}
    \begin{aligned}
      \sum_{i = 0}^m\sum_{j = 0}^n\max\{0, i + j - x\} 
      &= 
      \dots
    \end{aligned}
  \end{equation}
\end{document}